ADTExamples/QueryStructure/ProcessScheduler/TreeBasedRefinement.v
@@ -20,16 +20,11 @@ Unset Implicit Arguments.
 Module GenericTreeDB := FMapAVL.Make(Nat_as_OT). (* TODO: Add the generic implementation *)
 (*Module Import DBExtraFacts := FMapExtensions GenericTreeDB.*)
 
-Definition PIDIndex : @BagPlusBagProof (@Tuple ProcessSchema).
-Proof.
+Definition StatePIDIndexedTree : @BagPlusBagProof (@Tuple ProcessSchema).
   mkIndex ProcessSchema [STATE; PID].
 Defined.
 
-(* TODO: Remove: Definition PIDIndexedTree := BagType PIDIndex. *)
-
-(* TODO: Rename BagPlusBagProof to BagSpecification *)
-
-Definition Storage := AddCachingLayer (BagProof PIDIndex) (fun p => p PID)
+Definition Storage := AddCachingLayer (BagProof StatePIDIndexedTree) (fun p => p PID)
                                       0 max (ListMax_cacheable 0).
 
 Definition StorageType           := BagType Storage.
@@ -39,43 +34,6 @@ Definition StorageSearchTermType := SearchTermType Storage.
 Section TreeBasedRefinement.
   Open Scope type_scope.
   Open Scope Tuple_scope.
-
-  Definition NeatDB := StorageType.
-
-  Definition NeatDB_equivalence old_rep (neat_db: NeatDB) :=
-    let set_db := GetUnConstrRelation old_rep PROCESSES in
-    EnsembleListEquivalence set_db (benumerate neat_db).
-
-  Definition ObservationalEq {A B} f g :=
-    forall (a: A), @eq B (f a) (g a).
-
-  Lemma filter_by_equiv :
-    forall {A} f g,
-      ObservationalEq f g ->
-      forall seq, @List.filter A f seq = @List.filter A g seq.
-  Proof.
-    intros A f g obs seq; unfold ObservationalEq in obs; induction seq; simpl; try rewrite obs; try rewrite IHseq; trivial.
-  Qed.
-
-  Lemma filter_on_key :
-    forall (tree: StorageType) (key: nat),
-      SetEq
-        (List.filter
-           (fun (p: Process) => beq_nat (p PID) key)
-           (benumerate tree))
-        (bfind tree (None, (Some key, bstar))).
-  Proof.
-    intros tree key.
-
-    rewrite (filter_by_equiv _ (@bfind_matcher _ _ _ StorageIsBag (None, (Some key, bstar)))).
-    apply (bfind_correct).
-    
-    unfold ObservationalEq.
-    simpl.
-    intros.
-    rewrite (NatTreeExts.KeyFilter_beq beq_nat) by apply NPeano.Nat.eqb_spec.
-    rewrite andb_true_r; unfold cast; trivial.
-  Qed.
 
   Notation "x '∈' y" := (In _ y x) (at level 50, no associativity).
 
@@ -117,14 +75,6 @@ Section TreeBasedRefinement.
     intros; exfalso; apply (no_collisions_when_using_a_fresh_pid pid c _ _ H1); trivial.
   Qed.
 
-  Lemma tupleAgree_sym :
-    forall (heading: Heading) tup1 tup2 attrs,
-      @tupleAgree heading tup1 tup2 attrs <-> @tupleAgree heading tup2 tup1 attrs.
-  Proof.
-    intros; unfold tupleAgree.
-    intuition; symmetry; intuition.
-  Qed.
-
   Lemma insert_always_happens' :
     forall pid c,
       (forall a, (GetUnConstrRelation c PROCESSES) a -> pid > (a PID)) ->
@@ -146,17 +96,6 @@ Section TreeBasedRefinement.
     intros; exfalso; rewrite tupleAgree_sym in H1; apply (no_collisions_when_using_a_fresh_pid pid c _ _ H1); trivial.
   Qed.
 
-  Lemma get_update_unconstr_iff :
-    forall db_schema qs table new_contents,
-    forall x,
-      x ∈ GetUnConstrRelation (UpdateUnConstrRelation db_schema qs table new_contents) table <->
-      x ∈ new_contents.
-  Proof.
-    unfold GetUnConstrRelation, UpdateUnConstrRelation, RelationInsert;
-    intros; rewrite ith_replace_BoundIndex_eq;
-    reflexivity.
-  Qed.
-
   Lemma NeatScheduler :
     Sharpened ProcessSchedulerSpec.
   Proof.
@@ -164,27 +103,22 @@ Section TreeBasedRefinement.
 
     unfold ForAll_In; start honing QueryStructure.
 
-    hone representation using NeatDB_equivalence.
-    
-    (* (* TODO: Why does adding this followed simpl break the 
-          Equivalent_UnConstr_In_EnsembleListEquivalence rewrite? *) 
-      unfold UnConstrQuery_In.
-     (*simpl.*) *)
+    Definition equivalence := fun set_db (db: StorageType) =>
+      EnsembleListEquivalence (GetUnConstrRelation set_db PROCESSES) (benumerate db).
 
+    hone representation using equivalence. (* TODO: unfolding equiv here slows everything down. Why? *)
+    
     hone constructor INIT. {
-      unfold NeatDB_equivalence, DropQSConstraints_SiR.
       repeat setoid_rewrite refineEquiv_pick_ex_computes_to_and.
       repeat setoid_rewrite refineEquiv_pick_eq'.
       simplify with monad laws.
 
-      rewrite refine_pick_val;
-        [ | instantiate (1 := bempty); apply EnsembleListEquivalence_Empty ].
-
+      rewrite (refine_pick_val' bempty) by apply EnsembleListEquivalence_Empty.
       subst_body; higher_order_1_reflexivity. 
     }
 
     hone method ENUMERATE. {
-      unfold NeatDB_equivalence in H.
+      unfold equivalence in H.
 
       setoid_rewrite refineEquiv_pick_ex_computes_to_and.
       setoid_rewrite refineEquiv_pick_pair.
@@ -192,11 +126,11 @@ Section TreeBasedRefinement.
       simplify with monad laws.
       simpl.
 
-      rewrite (Equivalent_UnConstr_In_EnsembleListEquivalence);
-        eauto. (* TODO: Could explicitly pass the right list *)
+      rewrite (Equivalent_UnConstr_In_EnsembleListEquivalence) by eassumption.
 
       setoid_rewrite Equivalent_List_In_Where.
 
+      (* Full qualification of bfind_matcher needed to avoid apparition of spurious existentials *)
       rewrite (filter_by_equiv dec (@bfind_matcher _ _ _ StorageIsBag (Some n, (None, []))))
         by (
             unfold ObservationalEq; simpl; 
@@ -228,7 +162,7 @@ Section TreeBasedRefinement.
     (* TODO: The insert_always_happens scripts could probably be made more generic *)
     
     hone method GET_CPU_TIME. {
-      unfold NeatDB_equivalence in H.
+      unfold equivalence in H.
       
       setoid_rewrite refineEquiv_pick_ex_computes_to_and.
       setoid_rewrite refineEquiv_pick_pair.
@@ -236,10 +170,9 @@ Section TreeBasedRefinement.
       simplify with monad laws.
       simpl.
 
-      rewrite (Equivalent_UnConstr_In_EnsembleListEquivalence);
-        eauto. (* TODO: Could explicitly pass the right list *)
-
+      rewrite (Equivalent_UnConstr_In_EnsembleListEquivalence) by eassumption.
       setoid_rewrite Equivalent_List_In_Where.
+
       rewrite (filter_by_equiv dec (@bfind_matcher _ _ _ StorageIsBag (None, (Some n, [])))) 
         by (
             unfold ObservationalEq; simpl; 
@@ -260,7 +193,7 @@ Section TreeBasedRefinement.
     }
 
     hone method SPAWN. {
-      unfold NeatDB_equivalence in H.
+      unfold equivalence in H.
       
       setoid_rewrite refineEquiv_pick_ex_computes_to_and.
       setoid_rewrite refineEquiv_pick_pair.
@@ -288,10 +221,10 @@ Section TreeBasedRefinement.
       rewrite insert_always_happens' by eassumption.
       simplify with monad laws.
 
-      unfold NeatDB_equivalence.
+      unfold equivalence.
 
-      rewrite refine_pick_val;
-        [ | instantiate (1 := (binsert r_n <PID_COLUMN :: (S (ccached_value r_n)), STATE_COLUMN :: SLEEPING, CPU_COLUMN :: 0>))].
+      rewrite (refine_pick_val' 
+                 (binsert r_n <PID_COLUMN :: (S (ccached_value r_n)), STATE_COLUMN :: SLEEPING, CPU_COLUMN :: 0>)).
 
       simplify with monad laws.
 
